ok

SStructTT/SStruct/Erasure/Step.lean
@@ -19,85 +19,88 @@ inductive Value : Tm Srt -> Prop where
   | null : Value .null
 
 @[scoped aesop safe [constructors]]
-inductive Step0 : Tm Srt -> Tm Srt -> Prop where
+inductive Drop : Tm Srt -> Tm Srt -> Prop where
   | app_M {m m'} n :
-    Step0 m m' ->
-    Step0 (.app m n) (.app m' n)
+    Drop m m' ->
+    Drop (.app m n) (.app m' n)
   | app_N m {n n'} :
-    Step0 n n' ->
-    Step0 (.app m n) (.app m n')
+    Drop n n' ->
+    Drop (.app m n) (.app m n')
   | tup_M {m m'} n s :
-    Step0 m m' ->
-    Step0 (.tup m n s) (.tup m' n s)
+    Drop m m' ->
+    Drop (.tup m n s) (.tup m' n s)
   | tup_N m {n n'} s :
-    Step0 n n' ->
-    Step0 (.tup m n s) (.tup m n' s)
+    Drop n n' ->
+    Drop (.tup m n s) (.tup m n' s)
   | prj_M {m m'} n :
-    Step0 m m' ->
-    Step0 (.prj m n) (.prj m' n)
+    Drop m m' ->
+    Drop (.prj m n) (.prj m' n)
   | ite_M {m m'} n1 n2 :
-    Step0 m m' ->
-    Step0 (.ite m n1 n2) (.ite m' n1 n2)
+    Drop m m' ->
+    Drop (.ite m n1 n2) (.ite m' n1 n2)
   | drop_elim m n :
-    Step0 (.drop m n) n
+    Drop (.drop m n) n
 
 @[scoped aesop safe [constructors]]
-inductive Step1 : Tm Srt -> Tm Srt -> Prop where
+inductive CoreStep : Tm Srt -> Tm Srt -> Prop where
   | app_M {m m'} n :
-    Step1 m m' ->
-    Step1 (.app m n) (.app m' n)
+    CoreStep m m' ->
+    CoreStep (.app m n) (.app m' n)
   | app_N m {n n'} :
-    Step1 n n' ->
-    Step1 (.app m n) (.app m n')
+    CoreStep n n' ->
+    CoreStep (.app m n) (.app m n')
   | beta m n s :
     Value n ->
-    Step1 (.app (.lam m s) n) m.[n/]
+    CoreStep (.app (.lam m s) n) m.[n/]
   | tup_M {m m'} n s :
-    Step1 m m' ->
-    Step1 (.tup m n s) (.tup m' n s)
+    CoreStep m m' ->
+    CoreStep (.tup m n s) (.tup m' n s)
   | tup_N m {n n'} s :
-    Step1 n n' ->
-    Step1 (.tup m n s) (.tup m n' s)
+    CoreStep n n' ->
+    CoreStep (.tup m n s) (.tup m n' s)
   | prj_M {m m'} n :
-    Step1 m m' ->
-    Step1 (.prj m n) (.prj m' n)
+    CoreStep m m' ->
+    CoreStep (.prj m n) (.prj m' n)
   | prj_elim {m1 m2} n {s} :
     Value (.tup m1 m2 s) ->
-    Step1 (.prj (.tup m1 m2 s) n) n.[m2,m1/]
+    CoreStep (.prj (.tup m1 m2 s) n) n.[m2,m1/]
   | ite_M {m m'} n1 n2 :
-    Step1 m m' ->
-    Step1 (.ite m n1 n2) (.ite m' n1 n2)
+    CoreStep m m' ->
+    CoreStep (.ite m n1 n2) (.ite m' n1 n2)
   | ite_tt n1 n2 :
-    Step1 (.ite .tt n1 n2) n1
+    CoreStep (.ite .tt n1 n2) n1
   | ite_ff n1 n2 :
-    Step1 (.ite .ff n1 n2) n2
+    CoreStep (.ite .ff n1 n2) n2
   | rw_elim m :
-    Step1 (.rw m) m
+    CoreStep (.rw m) m
+
+abbrev Drops (m m' : Tm Srt) : Prop := Star Drop m m'
 
 inductive Step (m : Tm Srt) : Tm Srt -> Prop where
-  | intro {m' n} : Star Step0 m m' -> Step1 m' n -> Step m n
+  | intro {m' n} : Drops m m' -> CoreStep m' n -> Step m n
 
 notation:50 m:50 " ~>> " n:50 => Step m n
 notation:50 m:50 " ~>>* " n:50 => ARS.Star Step m n
 
-lemma Red0.var_inv {x} {t : Tm Srt} :
-    Star Step0 (.var x) t -> t = .var x := by
+lemma Drops.var_inv {x} {t : Tm Srt} :
+    Drops (.var x) t -> t = .var x := by
   intro rd; induction rd
   case R => simp
   case SE st ih =>
     subst_vars; cases st
 
-lemma Red0.lam_inv {m t : Tm Srt} {s} :
-    Star Step0 (.lam m s) t -> t = .lam m s := by
+lemma Drops.lam_inv {m t : Tm Srt} {s} :
+    Drops (.lam m s) t -> t = .lam m s := by
   intro rd; induction rd
   case R => simp
   case SE st e => subst_vars; cases st
 
-lemma Red0.app_inv {m n t : Tm Srt} :
-    Star Step0 (.app m n) t ->
-    ∃ m' n', t = .app m' n' ∧ Star Step0 m m' ∧ Star Step0 n n' := by
+lemma Drops.app_inv {m n t : Tm Srt} :
+    Drops (.app m n) t ->
+    ∃ m' n', t = .app m' n' ∧ Drops m m' ∧ Drops n n' := by
   intro rd; induction rd
-  case R => exists m, n; aesop
+  case R =>
+    exists m, n; aesop
   case SE st ih =>
     have ⟨m', n', e, rd1, rd2⟩  := ih
     subst_vars
@@ -111,9 +114,9 @@ lemma Red0.app_inv {m n t : Tm Srt} :
       . assumption
       . apply Star.SE rd2 st
 
-lemma Red0.tup_inv {m n t : Tm Srt} {s} :
-    Star Step0 (.tup m n s) t ->
-    ∃ m' n', t = .tup m' n' s ∧ Star Step0 m m' ∧ Star Step0 n n' := by
+lemma Drops.tup_inv {m n t : Tm Srt} {s} :
+    Drops (.tup m n s) t ->
+    ∃ m' n', t = .tup m' n' s ∧ Drops m m' ∧ Drops n n' := by
   intro rd; induction rd
   case R => exists m, n; aesop
   case SE st ih =>
@@ -129,9 +132,9 @@ lemma Red0.tup_inv {m n t : Tm Srt} {s} :
       . assumption
       . apply Star.SE rd2 st
 
-lemma Red0.prj_inv {m n t : Tm Srt} :
-    Star Step0 (.prj m n) t ->
-    ∃ m', t = .prj m' n ∧ Star Step0 m m' := by
+lemma Drops.prj_inv {m n t : Tm Srt} :
+    Drops (.prj m n) t ->
+    ∃ m', t = .prj m' n ∧ Drops m m' := by
   intro rd; induction rd
   case R => exists m; aesop
   case SE st ih =>
@@ -142,19 +145,19 @@ lemma Red0.prj_inv {m n t : Tm Srt} :
       exists mx; simp
       apply Star.SE rd st
 
-lemma Red0.tt_inv {t : Tm Srt} : Star Step0 .tt t -> t = .tt := by
+lemma Drops.tt_inv {t : Tm Srt} : Drops .tt t -> t = .tt := by
   intro rd; induction rd
   case R => simp
   case SE st ih => subst_vars; cases st
 
-lemma Red0.ff_inv {t : Tm Srt} : Star Step0 .ff t -> t = .ff := by
+lemma Drops.ff_inv {t : Tm Srt} : Drops .ff t -> t = .ff := by
   intro rd; induction rd
   case R => simp
   case SE st ih => subst_vars; cases st
 
-lemma Red0.ite_inv {m n1 n2 t : Tm Srt} :
-    Star Step0 (.ite m n1 n2) t ->
-    ∃ m', t = .ite m' n1 n2 ∧ Star Step0 m m' := by
+lemma Drops.ite_inv {m n1 n2 t : Tm Srt} :
+    Drops (.ite m n1 n2) t ->
+    ∃ m', t = .ite m' n1 n2 ∧ Drops m m' := by
   intro rd; induction rd
   case R => exists m; aesop
   case SE st ih =>
@@ -165,13 +168,13 @@ lemma Red0.ite_inv {m n1 n2 t : Tm Srt} :
       exists mx; simp
       apply Star.SE rd st
 
-lemma Red0.rw_inv {m t : Tm Srt} : Star Step0 (.rw m) t -> t = .rw m := by
+lemma Drops.rw_inv {m t : Tm Srt} : Drops (.rw m) t -> t = .rw m := by
   intro rd; induction rd
   case R => simp
   case SE st ih => subst_vars; cases st
 
-lemma Red0.drop_inv {m n a b : Tm Srt} :
-    Star Step0 (.drop m n) a -> Step0 a b -> Star Step0 n b := by
+lemma Drops.drop_inv {m n a b : Tm Srt} :
+    Drops (.drop m n) a -> Drop a b -> Drops n b := by
   intro rd st; induction rd generalizing b
   case R =>
     cases st
@@ -182,15 +185,15 @@ lemma Red0.drop_inv {m n a b : Tm Srt} :
       assumption
     . assumption
 
-lemma Red0.ptr_inv {l} {t : Tm Srt} :
-    Star Step0 (.ptr l) t -> t = .ptr l := by
+lemma Drops.ptr_inv {l} {t : Tm Srt} :
+    Drops (.ptr l) t -> t = .ptr l := by
   intro rd; induction rd
   case R => simp
   case SE st ih =>
     subst_vars; cases st
 
-lemma Red0.null_inv {t : Tm Srt} :
-    Star Step0 .null t -> t = .null := by
+lemma Drops.null_inv {t : Tm Srt} :
+    Drops .null t -> t = .null := by
   intro rd; induction rd
   case R => simp
   case SE st ih =>
