SStructTT/SStruct/Erasure/Normalize.lean
@@ -10,31 +10,25 @@ lemma Erased.value_step {m n : Tm Srt} :
   intro vl st; induction vl generalizing n
   case lam =>
     rcases st with ⟨rd, st⟩
-    rw[Red0.lam_inv rd] at st
-    cases st
+    rw[rd.lam_inv] at st; cases st
   case tup ihm ihn =>
     rcases st with ⟨rd, st⟩
-    have ⟨_, _, _, rd1, rd2⟩ := Red0.tup_inv rd
-    subst_vars
-    cases st
+    have ⟨_, _, _, rd1, rd2⟩ := rd.tup_inv
+    subst_vars; cases st
     case tup_M st => apply ihm (Step.intro rd1 st)
     case tup_N st => apply ihn (Step.intro rd2 st)
   case tt =>
     rcases st with ⟨rd, st⟩
-    rw[Red0.tt_inv rd] at st
-    cases st
+    rw[rd.tt_inv] at st; cases st
   case ff =>
     rcases st with ⟨rd, st⟩
-    rw[Red0.ff_inv rd] at st
-    cases st
+    rw[rd.ff_inv] at st; cases st
   case ptr =>
     rcases st with ⟨rd, st⟩
-    rw[Red0.ptr_inv rd] at st
-    cases st
+    rw[rd.ptr_inv] at st; cases st
   case null =>
     rcases st with ⟨rd, st⟩
-    rw[Red0.null_inv rd] at st
-    cases st
+    rw[rd.null_inv] at st; cases st
 
 variable [ord : SrtOrder Srt]
 
